sketch two transformation steps needed to use compiler correctness:
1) Change decode from RV32IM to RV32I (lemma run1_IM_to_I),
   based on an XAddrs/valid_machine hack to remain compatible
   with compiler's parameterization that's not aware of free monads,
   only works if compiler doesn't emit any M instructions
2) Change state representation from MetricRiscvMachine to State
   (with CSRs), based on induction on free monad

and wip combining these two with bedrock2 source program proof
and compiler correctness theorem

compiler/src/compilerExamples/SoftmulCompile.v
@@ -28,31 +28,130 @@ Require Import riscv.Utility.Encode.
 Require Import riscv.Proofs.EncodeBound.
 Require Import riscv.Platform.MinimalCSRs.
 Require Import riscv.Platform.MaterializeRiscvProgram.
+Require Import riscv.Platform.MetricMinimalNoMul.
 Require Import compiler.regs_initialized.
 Require Import compilerExamples.SoftmulBedrock2.
 Require compiler.Pipeline.
+Require Import bedrock2.BasicC32Semantics.
 Require Import bedrock2.SepAutoArray bedrock2.SepAuto.
 
 Section Riscv.
-  Context {word: Word.Interface.word 32}.
-  Context {word_ok: word.ok word}.
-  Context {Mem: map.map word byte}.
-  Context {Mem_ok: map.ok Mem}.
+  Import bedrock2.BasicC32Semantics.
   Context {registers: map.map Z word}.
   Context {registers_ok: map.ok registers}.
-
-  Add Ring wring : (word.ring_theory (word := word))
-      ((*This preprocessing is too expensive to be always run, especially if
-         we do many ring_simplify in a sequence, in which case it's sufficient
-         to run it once before the ring_simplify sequence.
-         preprocess [autorewrite with rew_word_morphism],*)
-       morphism (word.ring_morph (word := word)),
-       constants [word_cst]).
 
   (* RISC-V Monad *)
   Local Notation M := (free riscv_primitive primitive_result).
 
   Local Hint Mode map.map - - : typeclass_instances.
+
+  Instance RV32I_bitwidth: FlatToRiscvCommon.bitwidth_iset 32 RV32I.
+  Proof. reflexivity. Qed.
+
+  Lemma decode_IM_I_to_I: forall i inst,
+      decode RV32IM i = IInstruction inst ->
+      decode RV32I  i = IInstruction inst.
+  Proof.
+  Admitted.
+
+  Lemma decode_IM_Invalid_to_I: forall i z,
+      decode RV32IM i = InvalidInstruction z ->
+      decode RV32I  i = InvalidInstruction z.
+  Proof.
+  Admitted.
+
+  Lemma decode_IM_cases: forall z,
+      (exists iinst, decode RV32IM z = IInstruction iinst) \/
+      (exists minst, decode RV32IM z = MInstruction minst) \/
+      (decode RV32IM z = InvalidInstruction z).
+  Admitted.
+
+  (* To use the compiler correctness statement, we need to apply two transformation steps:
+     1) Change decode from RV32IM to RV32I (lemma run1_IM_to_I)
+     2) Change state representation from MetricRiscvMachine to State (with CSRs) *)
+
+  (* valid_machine contains the extra condition no_M saying that all executable addresses
+     are not an M instruction, which will only hold for certain input programs, and we
+     will check it instruction-by-instruction for the compiled softmul handler program,
+     in order to turn the compiler proof, which usually is about an execution on an RV32IM
+     machine into a statement about an execution on an RV32I machine. *)
+  Lemma run1_IM_to_I_run1: forall (initial: MetricRiscvMachine) post,
+      Primitives.valid_machine initial ->
+      GoFlatToRiscv.mcomp_sat (Run.run1 RV32IM) initial post ->
+      GoFlatToRiscv.mcomp_sat (Run.run1 RV32I) initial post.
+  Proof.
+    unfold Run.run1. cbn -[HList.tuple].
+    unfold MinimalNoMul.no_M, MinimalNoMul.load.
+    intros. fwd. split. 1: assumption.
+    replace (decode RV32I (LittleEndian.combine 4 t)) with
+      (decode RV32IM (LittleEndian.combine 4 t)). 1: assumption.
+    clear H0p1.
+    specialize (H0p0 eq_refl).
+    specialize (H _ _ H0p0 E).
+    destruct (decode_IM_cases (LittleEndian.combine 4 t)) as [ C | [C | C] ];
+      fwd; rewrite C; symmetry.
+    - eapply decode_IM_I_to_I. exact C.
+    - exfalso. eapply H. exact C.
+    - eapply decode_IM_Invalid_to_I. exact C.
+  Qed.
+
+  Lemma run1_IM_to_I: forall s post,
+      runsTo (GoFlatToRiscv.mcomp_sat (Run.run1 RV32IM)) s post ->
+      Primitives.valid_machine s ->
+      runsTo (GoFlatToRiscv.mcomp_sat (Run.run1 RV32I )) s post.
+  Proof.
+    induction 1; intros.
+    - eapply runsToDone. assumption.
+    - eapply runsToStep with (midset := fun m => midset m /\ Primitives.valid_machine m).
+      + eapply run1_IM_to_I_run1. 1: assumption.
+        eapply GoFlatToRiscv.mcomp_sat_weaken.
+        2: eapply GoFlatToRiscv.run1_get_sane.
+        2,3: eassumption.
+        1: intros mach A; exact A.
+        intros. fwd. auto.
+      + intros. fwd. eapply H1; assumption.
+  Qed.
+
+  Definition states_related(sH: MetricRiscvMachine)(sL: State): Prop :=
+    sH.(getRegs) = sL.(regs) /\
+    sH.(getPc) = sL.(pc) /\
+    sH.(getNextPc) = sL.(nextPc) /\
+    sH.(getMem) = sL.(MinimalCSRs.mem) /\
+    (* no constraints on sH.(getXAddrs) here *)
+    sH.(getLog) = [] /\ sL.(log) = [].
+
+  Lemma change_state_rep_primitive: forall a sH sL postH,
+      states_related sH sL ->
+      interp_action a sH postH ->
+      run_primitive a sL (fun a sL' =>
+         exists sH', states_related sH' sL' /\ postH a sH') (fun _ => False).
+  Proof.
+    pose proof Radd_comm word.ring_theory.
+    destruct a; intros; destruct sH as [sH logH]; destruct sH, sL;
+      unfold states_related, getReg, interp_action in *;
+      cbn -[Memory.load_bytes map.get] in *;
+      unfold load, store, MinimalNoMul.load, MinimalNoMul.store in *;
+      fwd; cbn -[Memory.load_bytes map.get] in *;
+      try contradiction;
+      try rewrite_match;
+      try (eexists {| getMachine := {| getRegs := _ |} |});
+      cbn -[map.get]; eauto 10.
+  Qed.
+
+  Lemma change_state_rep_free: forall A (m: M A) sH sL postH,
+      states_related sH sL ->
+      free.interp MetricMinimalNoMul.interp_action m sH postH ->
+      free.interpret run_primitive m sL (fun a sL' =>
+         exists sH', states_related sH' sL' /\ postH a sH') (fun _ => False).
+  Proof.
+    induction m; intros.
+    - cbn in *.
+      eapply weaken_run_primitive with (postA1 := fun _ => False). 2: auto.
+      2: eapply change_state_rep_primitive; eassumption.
+      cbv beta.
+      intros. fwd. eapply H; eauto.
+    - cbn in *. eauto.
+  Qed.
 
   Definition run1(decoder: Z -> Instruction): M unit :=
     pc <- getPC;
@@ -60,7 +159,37 @@ Section Riscv.
     Execute.execute (decoder (LittleEndian.combine 4 inst));;
     endCycleNormal.
 
-  Definition instr(decoder: Z -> Instruction)(inst: Instruction)(addr: word): Mem -> Prop :=
+  (* both the finish-postcondition and the abort-postcondition are set to `post`
+     to make sure `post` holds in all cases: *)
+  Definition mcomp_sat(m: M unit)(initial: State)(post: State -> Prop): Prop :=
+    free.interpret run_primitive m initial (fun tt => post) post.
+
+  Lemma change_state_rep: forall sH postH,
+      runsTo (GoFlatToRiscv.mcomp_sat (Run.run1 RV32I)) sH postH ->
+      forall sL, states_related sH sL ->
+      runsTo (mcomp_sat (run1 idecode)) sL (fun sL' =>
+         exists sH', states_related sH' sL' /\ postH sH').
+  Proof.
+    induction 1; intros.
+    - eapply runsToDone. eauto.
+    - eapply runsToStep.
+      + unfold mcomp_sat.
+        eapply free.interpret_weaken_post.
+        4: {
+          eapply change_state_rep_free. 1: eassumption.
+          unfold GoFlatToRiscv.mcomp_sat, Primitives.mcomp_sat,
+                 MetricMinimalNoMulPrimitivesParams in *.
+          exact H.
+        }
+        1: eapply weaken_run_primitive.
+        all: cbv beta; intros.
+        2: contradiction.
+        exact H3.
+      + cbv beta; intros.
+        fwd. eauto.
+  Qed.
+
+  Definition instr(decoder: Z -> Instruction)(inst: Instruction)(addr: word): mem -> Prop :=
     ex1 (fun z => sep (addr |-> truncated_scalar access_size.four z)
                       (emp (decoder z = inst /\ 0 <= z < 2 ^ 32))).
 
@@ -68,35 +197,27 @@ Section Riscv.
   Open Scope array_abbrevs_scope.
   Notation "'program' d" := (array (instr d) 4) (at level 10): array_abbrevs_scope.
 
-  (* both the finish-postcondition and the abort-postcondition are set to `post`
-     to make sure `post` holds in all cases: *)
-  Definition mcomp_sat(m: M unit)(initial: State)(post: State -> Prop): Prop :=
-    free.interpret run_primitive m initial (fun tt => post) post.
-
-  Import RegisterNames PseudoInstructions.
-  Import InstructionCoercions. Open Scope ilist_scope.
-  Import Decode.
-
-  (* a3 := a1 * a2
-     without using mul, but with a naive loop:
-     a3 := 0;
-     while (0 != a1) {
-       a3 := a3 + a2;
-       a1 := a1 - 1;
-     } *)
-  Definition softmul_insts := [[
-    Addi a3 zero 0;
-    Beq zero a1 16;
-    Add a3 a3 a2;
-    Addi a1 a1 (-1);
-    J (-12)
-  ]].
-
   Definition funimplsList := softmul :: rpmul.rpmul :: nil.
   Definition prog := map.of_list funimplsList.
 
-  Instance RV32I_bitwidth: FlatToRiscvCommon.bitwidth_iset 32 RV32I.
-  Proof. reflexivity. Qed.
+  Lemma funs_valid: ExprImp.valid_funs (map.of_list funimplsList).
+  Proof.
+    unfold ExprImp.valid_funs, ExprImp.valid_fun.
+    intros.
+    set (funnames := (List.map fst funimplsList)). cbv in funnames.
+    destruct (List.In_dec String.string_dec f funnames).
+    - subst funnames. simpl in i.
+      repeat destruct i as [i | i]; try contradiction; subst f; vm_compute in H; fwd; split;
+        repeat constructor; intro C; simpl in C; intuition discriminate.
+    - exfalso. apply n; clear n.  change funnames with (List.map fst funimplsList).
+      clear funnames.
+      generalize dependent funimplsList. induction l; intros.
+      + simpl in H. discriminate.
+      + destruct a. unfold map.of_list in H. rewrite map.get_put_dec in H.
+        destruct_one_match_hyp.
+        * fwd. subst. simpl. auto.
+        * simpl. right. eapply IHl. exact H.
+  Qed.
 
   (* TODO implement in bedrock2 and compile to riscv, and also need to prove that
      programs running on the RISC-V machine used by the compiler (without CSRs)
@@ -111,18 +232,46 @@ Section Riscv.
   Defined.
 
   Definition mul_insts: list Instruction := Eval compute in fst (fst mul_insts_tuple).
+  Definition mul_insts_fpos: SortedListString.map (nat * nat * Z) :=
+    Eval compute in snd (fst mul_insts_tuple).
+  Definition mul_insts_req_stack: Z := Eval compute in snd (mul_insts_tuple).
+
+  Lemma mul_insts_result_eq:
+    mul_insts_result = Result.Success (mul_insts, mul_insts_fpos, mul_insts_req_stack).
+  Proof. vm_compute. reflexivity. Qed.
+
+  Definition no_M_insts: list Instruction -> bool :=
+    List.forallb (fun i => match i with
+                           | MInstruction _ => false
+                           | _ => true
+                           end).
+
+  Lemma no_M_from_I_sep: forall (mach: RiscvMachine) insts R,
+      sep (mach.(getPc) |-> program idecode insts) R mach.(getMem) ->
+      mach.(getXAddrs) = List.unfoldn (word.add (word.of_Z 1))
+                                      (4 * Datatypes.length insts) mach.(getPc) ->
+      MinimalNoMul.no_M mach.
+  Admitted.
+
+  Lemma link_softmul_bedrock2: spec_of_softmul funimplsList.
+  Proof.
+    eapply softmul_ok. eapply rpmul.rpmul_ok.
+  Qed.
+
+  Axiom TODO: False.
 
   (* TODO will need some stack space *)
   Lemma mul_correct: forall initial a_regs regvals invalidIInst R (post: State -> Prop)
                             ret_addr sp_val rd rs1 rs2,
       initial.(nextPc) = word.add initial.(pc) (word.of_Z 4) ->
-      map.get initial.(regs) RegisterNames.a0 = Some (word.of_Z invalidIInst) ->
+      initial.(log) = [] ->
+      map.get initial.(regs) RegisterNames.a0 = Some invalidIInst ->
       map.get initial.(regs) RegisterNames.a1 = Some a_regs ->
       map.get initial.(regs) RegisterNames.ra = Some ret_addr ->
       map.get initial.(regs) RegisterNames.sp = Some sp_val ->
-      mdecode invalidIInst = MInstruction (Mul rd rs1 rs2) ->
+      mdecode (word.unsigned invalidIInst) = MInstruction (Mul rd rs1 rs2) ->
       seps [a_regs |-> word_array regvals; initial.(pc) |-> program idecode mul_insts; R]
-           initial.(mem) /\
+           initial.(MinimalCSRs.mem) /\
       (forall newMem newRegs,
         seps [a_regs |-> word_array (List.upd regvals (Z.to_nat rd) (word.mul
                    (List.nth (Z.to_nat rs1) regvals default)
@@ -131,10 +280,76 @@ Section Riscv.
         map.get newRegs RegisterNames.sp = Some sp_val ->
         post { initial with pc := ret_addr;
                             nextPc := word.add ret_addr (word.of_Z 4);
-                            mem := newMem;
+                            MinimalCSRs.mem := newMem;
                             regs := newRegs (* <- regs arbitrarily changed except sp *)
                             (* log and csrs remain the same *) }) ->
       runsTo (mcomp_sat (run1 idecode)) initial post.
+  Proof.
+    intros. destruct H6 as [ML C].
+    eapply runsTo_weaken.
+    { eapply change_state_rep with (sH := {|
+            (****************)
+        getMachine := {|
+          getRegs := initial.(regs);
+          getPc := initial.(pc);
+          getNextPc := initial.(nextPc);
+          getMem := initial.(MinimalCSRs.mem);
+          getXAddrs := List.unfoldn (word.add (word.of_Z 1)) (4 * List.length mul_insts)
+                                    initial.(pc);
+          getLog := []
+        |};
+        getMetrics := MetricLogging.EmptyMetricLog
+      |}).
+      2: {
+        unfold states_related; cbn -[array HList.tuple] in *.
+        ssplit; congruence.
+      }
+      eapply run1_IM_to_I.
+            (************)
+      2: {
+        unfold Primitives.valid_machine, MetricMinimalNoMulPrimitivesParams.
+        eapply no_M_from_I_sep;
+        cbn -[array HList.tuple List.unfoldn List.length Nat.mul load_bytes].
+        2: reflexivity. cbn [seps] in ML. ecancel_assumption.
+      }
+      eapply (Pipeline.compiler_correct_wp (ext_spec := fun _ _ _ _ _ => False)).
+             (****************************)
+      5: {
+        pose proof mul_insts_result_eq as P. unfold mul_insts_result in P.
+        exact P.
+      }
+      { clear C.
+        unfold FlatToRiscvCommon.compiles_FlatToRiscv_correctly.
+        intros. inversion H6. contradiction. }
+      { intros. reflexivity. }
+      { exact funs_valid. }
+      { constructor.
+        - intro A. inversion A; try discriminate. eapply in_nil. eassumption.
+        - constructor. 2: constructor. intro B. eapply in_nil. eassumption. }
+      {
+        pose proof link_softmul_bedrock2 as P.
+                  (*********************)
+        unfold spec_of_softmul in P.
+        eapply P; clear P.
+        split.
+        - eassumption.
+        - case TODO. (* separation logic splitting high-level mem out of whole mem *) }
+      { reflexivity. }
+      { case TODO. (* needs stack space *) }
+      { case TODO. (* stack related *) }
+      { cbn -[array HList.tuple Datatypes.length]. instantiate (1 := pc initial).
+        ring. }
+      { cbn -[array HList.tuple Datatypes.length]. eassumption. }
+      { case TODO. (*   word.unsigned ret_addr mod 4 = 0 *) }
+      { cbn -[array HList.tuple Datatypes.length]. unfold a0, a1 in *. rewrite_match.
+        reflexivity. }
+      { cbn -[array HList.tuple Datatypes.length]. reflexivity. }
+      { case TODO. (* machine_ok... *) } }
+    { cbv beta. cbn -[array HList.tuple Datatypes.length].
+      intros. fwd.
+      case TODO. (* postcondition matching... *) }
+    Unshelve.
+    all: case TODO.
   Admitted.
 
   (* Needed if the handler wants to handle the case where the instruction is not
@@ -144,14 +359,14 @@ Section Riscv.
       map.get initial.(regs) RegisterNames.a0 = Some invalidIInst ->
       map.get initial.(regs) RegisterNames.a1 = Some a_regs ->
       seps [a_regs |-> word_array regvals; initial.(pc) |-> program idecode mul_insts; R]
-           initial.(mem) /\
+           initial.(MinimalCSRs.mem) /\
       (forall final,
         ((* case 1: It was not the Mul instruction *)
          (map.get final.(regs) RegisterNames.a0 = Some (word.of_Z 0) /\
           (forall rd rs1 rs2, decode RV32IM (word.unsigned invalidIInst) <>
                                 MInstruction (Mul rd rs1 rs2)) /\
           seps [a_regs |-> word_array regvals;
-                initial.(pc) |-> program idecode mul_insts; R] final.(mem))
+                initial.(pc) |-> program idecode mul_insts; R] final.(MinimalCSRs.mem))
          \/ (* case 2: It was the Mul instruction *)
          (exists ans rd rs1 rs2 v1 v2,
           map.get final.(regs) RegisterNames.a0 = Some ans /\
@@ -160,7 +375,7 @@ Section Riscv.
           nth_error regvals (Z.to_nat rs1) = Some v1 /\
           nth_error regvals (Z.to_nat rs2) = Some v2 /\
           seps [a_regs |-> word_array (List.upd regvals (Z.to_nat rd) (word.mul v1 v2));
-               initial.(pc) |-> program idecode mul_insts; R] final.(mem))) ->
+               initial.(pc) |-> program idecode mul_insts; R] final.(MinimalCSRs.mem))) ->
         (* In common: *)
         final.(pc) = word.add initial.(pc) (word.mul (word.of_Z 4)
                            (word.of_Z (Z.of_nat (List.length mul_insts)))) ->
